haskabelle/thy/TestingMappingFunStatelessCircus.thy
@@ -10,8 +10,8 @@ where
 | "\<Omega> CSPChaos = CSPChaos"
 | "\<Omega> (CSPSeq ca cb) = (CSPSeq (\<Omega> ca) (\<Omega> cb))"
 | "\<Omega> (CSPExtChoice ca cb) 
-    = (let lsx = (map fst (remdups (set_to_list (abs_fv_CAction (CSPExtChoice ca cb)))))
-       in make_get_com lsx (abs_rename_vars_CAction (CSPExtChoice (\<Omega>' ca) (\<Omega>' cb))))"
+    = (let lsx = (map fst (abs_remdups (abs_free_var_CAction (CSPExtChoice ca cb))))
+       in abs_make_get_com lsx (abs_rename_vars_CAction (CSPExtChoice (\<Omega>' ca) (\<Omega>' cb))))"
 | "\<Omega> x = x"
 | "\<Omega>' CSPSkip = CSPSkip"
 | "\<Omega>' CSPStop = CSPStop"
@@ -19,16 +19,31 @@ where
 | "\<Omega>' (CSPSeq ca cb) = (CSPSeq (\<Omega>' ca) (\<Omega>' cb))"
 | "\<Omega>' x = \<Omega> x"
 
-lemma "set_to_list {} = []"
-   by (meson finite.emptyI set_empty set_set_to_list)
-
-lemma "a1 = CSPSkip \<and> a2 = CSPSkip \<Longrightarrow> \<Omega> (CSPExtChoice a1 a2) = omega_CAction (CSPExtChoice a1 a2)"
-  apply simp
-  by (metis Domain_empty OmegaDefs.remdups.simps(1) finite.emptyI fst_eq_Domain make_get_com.simps(3) set_empty set_map set_set_to_list)
-
-lemma "a1 = CSPSkip \<and> a2 = CSPSkip \<Longrightarrow> \<Omega> (CSPSeq a1 a2) = omega_CAction  (CSPSeq a1 a2)"
- by simp
+lemma "a1 = CSPSkip \<and> a2 = CSPSkip \<Longrightarrow> \<Omega> (CSPExtChoice a1 a2) = omega_CAction (CSPExtChoice a1 a2)" by simp
     
+lemma "a1 = CSPSkip \<and> a2 = CSPSkip \<Longrightarrow> \<Omega> (CSPSeq a1 a2) = omega_CAction  (CSPSeq a1 a2)" by simp
+lemma thm_omega_prime:"\<Omega>' a = omega_prime_CAction a"
+proof (induction a)
+  case CSPSkip
+  then show ?case by simp
+next
+  case CSPStop
+  then show ?case  by simp
+next
+  case CSPChaos
+  then show ?case  by simp
+next
+  case (CSPCommAction x1 a)
+  then show ?case by simp
+next
+  case (CSPSeq a1 a2)
+  then show ?case  by simp
+next
+  case (CSPExtChoice a1 a2)
+  then show ?case 
+    by (simp add: thm_rv_CAction thm_make_get_com thm_free_var_CAction thm_remdups)
+qed
+      
 lemma "\<Omega> a = omega_CAction a"
 proof (induction a)
   case CSPSkip
@@ -47,7 +62,8 @@ next
   then show ?case  by simp
 next
   case (CSPExtChoice a1 a2)
-  then show ?case sorry   
+  then show ?case 
+    by (simp add: thm_omega_prime thm_rv_CAction thm_make_get_com thm_free_var_CAction thm_remdups)
 qed
   
 end
